Logic/Modal/Standard/Kripke/Completeness.lean
@@ -1,6 +1,188 @@
 import Logic.Modal.Standard.Deduction
 import Logic.Modal.Standard.Kripke.Semantics
+import Logic.Propositional.Superintuitionistic.Kripke.Completeness
 
-namespace LO.Modal.Standard.Kripke
+namespace LO.System
 
-end LO.Modal.Standard.Kripke
+variable {F : Type*} [LogicalConnective F] [DecidableEq F]
+variable {S : Type*} [System F S]
+variable {𝓢 : S}
+variable [Minimal 𝓢]
+
+lemma dhyp! (q : F) (b : 𝓢 ⊢! p) : 𝓢 ⊢! q ⟶ p := ⟨dhyp q b.some⟩
+
+namespace Context
+
+lemma by_axm! {p} (h : p ∈ Γ) : Γ *⊢[𝓢]! p := by
+  apply provable_iff.mpr;
+  existsi {p};
+  constructor;
+  . intro q hq; have := Finset.mem_singleton.mp hq; subst_vars; simpa;
+  . exact FiniteContext.by_axm! (by tauto)
+
+end Context
+
+end LO.System
+
+
+namespace LO.Modal.Standard
+
+variable [DecidableEq α]
+
+@[simp]
+def Theory.ΛConsistent (Λ : AxiomSet α) (T : Theory α) := ∀ Γ : List (Formula α), (∀ p ∈ Γ, p ∈ T) → Λ ⊬! Γ.conj ⟶ ⊥
+notation:max "(" Λ ")-Consistent " T:90 => Theory.ΛConsistent Λ T
+
+variable {Λ : AxiomSet α}
+variable {T : Theory α} (consisT : (Λ)-Consistent T)
+
+open System
+open Theory
+
+namespace Theory
+
+variable (consisT : (Λ)-Consistent T)
+
+lemma not_provable_falsum : Λ ⊬! ⊥ := by
+  by_contra hC;
+  have : Λ ⊢! ⊤ ⟶ ⊥ := dhyp! ⊤ hC;
+  have : Λ ⊬! ⊤ ⟶ ⊥ := by simpa [Finset.conj] using consisT ∅ (by simp);
+  contradiction;
+
+lemma not_mem_falsum_of_Λconsistent : ⊥ ∉ T := by
+  by_contra hC;
+  have : Λ ⊬! ⊥ ⟶ ⊥ := implyLeftConjSingleton!.not.mp $ consisT _ (by simpa);
+  have : Λ ⊢! ⊥ ⟶ ⊥ := efq!;
+  contradiction;
+
+end Theory
+
+lemma exists_maximal_consistent_theory :
+  ∃ Z, (Λ)-Consistent Z ∧ T ⊆ Z ∧ ∀ U, (Λ)-Consistent U → Z ⊆ U → U = Z
+  := zorn_subset_nonempty { T : Theory α | (Λ)-Consistent T } (by
+    intro c hc chain hnc;
+    existsi (⋃₀ c);
+    simp only [ΛConsistent, Set.mem_setOf_eq, Set.mem_sUnion];
+    constructor;
+    . by_contra hC;
+      obtain ⟨Γ, hΓs, hΓd⟩ := by simpa using hC;
+      obtain ⟨U, hUc, hUs⟩ :=
+        Set.subset_mem_chain_of_finite c hnc chain
+          (s := ↑Γ.toFinset) (by simp)
+          (by intro p hp; simp_all);
+      simp [List.coe_toFinset] at hUs;
+      have : (Λ)-Consistent U := hc hUc;
+      have : ¬(Λ)-Consistent U := by
+        simp only [ΛConsistent, not_forall, not_not, exists_prop];
+        existsi Γ;
+        constructor;
+        . intro p hp; exact hUs hp;
+        . assumption;
+      contradiction;
+    . intro s a;
+      exact Set.subset_sUnion_of_mem a;
+  ) T consisT
+
+structure MaximalConsistentByTheory (Λ : AxiomSet α) where
+  theory : Theory α
+  consistent : (Λ)-Consistent theory
+  maximal : ∀ {U}, theory ⊂ U → ¬(Λ)-Consistent U
+
+alias MCT := MaximalConsistentByTheory
+
+namespace MaximalConsistentByTheory
+
+variable {Ω Ω₁ Ω₂ : MCT Λ}
+variable {p : Formula α}
+
+@[simp]
+lemma unprovable_falsum : Ω.theory *⊬[Λ]! ⊥ := by
+  have := Theory.not_provable_falsum Ω.consistent;
+  by_contra hC;
+  have := Context.provable_iff.mp hC;
+  sorry;
+
+lemma membership_iff : (p ∈ Ω.theory) ↔ (Ω.theory *⊢[Λ]! p) := by
+  constructor;
+  . intro h; exact Context.by_axm! h;
+  . intro hp;
+    suffices ~p ∉ Ω.theory by sorry;
+    by_contra hC;
+    have hnp : Ω.theory *⊢[Λ]! ~p := Context.by_axm! hC;
+    have : Ω.theory *⊢[Λ]! ⊥ := hnp ⨀ hp;
+    have : Ω.theory *⊬[Λ]! ⊥ := unprovable_falsum;
+    contradiction;
+
+lemma iff_congr : (Ω.theory *⊢[Λ]! (p ⟷ q)) → ((p ∈ Ω.theory) ↔ (q ∈ Ω.theory)) := by
+  simp only [LogicalConnective.iff];
+  intro hpq;
+  constructor;
+  . intro hp;
+    exact membership_iff.mpr $ (conj₁'! hpq) ⨀ (membership_iff.mp hp)
+  . intro hq;
+    exact membership_iff.mpr $ (conj₂'! hpq) ⨀ (membership_iff.mp hq)
+
+lemma mem_dn_iff : (p ∈ Ω.theory) ↔ (~~p ∈ Ω.theory) := iff_congr $ (by sorry)
+
+end MaximalConsistentByTheory
+
+lemma exists_maximal_consistented_theory : ∃ (Ω : MCT Λ), (T ⊆ Ω.theory) := by
+  have ⟨Ω, hΩ₁, hΩ₂, hΩ₃⟩ := exists_maximal_consistent_theory consisT;
+  existsi ⟨
+    Ω,
+    hΩ₁,
+    by
+      rintro U ⟨hU₁, hU₂⟩;
+      by_contra hC;
+      have : U = Ω := hΩ₃ U hC hU₁;
+      subst_vars;
+      simp at hU₂;
+  ⟩;
+  simp_all only [ΛConsistent];
+
+alias lindenbaum := exists_maximal_consistented_theory
+
+open Formula
+
+namespace Kripke
+
+def CanonicalModel (Λ : AxiomSet α) : Model (MCT Λ) α where
+  frame (Ω₁ Ω₂) := □⁻¹Ω₁.theory ⊆ Ω₂.theory
+  valuation Ω a := (atom a) ∈ Ω.theory
+
+namespace CanonicalModel
+
+lemma frame_def: (CanonicalModel Λ).frame Ω₁ Ω₂ ↔ (∀ {p : Formula α}, □p ∈ Ω₁.theory → p ∈ Ω₂.theory) := by rfl
+
+@[simp]
+lemma val_def {a : α} : (CanonicalModel Λ).valuation Ω a ↔ (atom a) ∈ Ω.theory := by rfl
+
+end CanonicalModel
+
+lemma truthlemma {p : Formula α} : ∀ {Ω : MCT Λ}, ((CanonicalModel Λ, Ω) ⊧ p) ↔ (p ∈ Ω.theory) := by
+  sorry;
+  /-
+  induction p using Formula.rec' with
+  | hatom => simp;
+  | hfalsum => simp;
+  | himp => simp_all [imp_membership_iff'];
+  | hor => simp_all [or_membership_iff];
+  | hand => simp_all [and_membership_iff];
+  | hbox p ih =>
+    intro Ω;
+    constructor;
+    . intro h;
+      apply (mct_mem_box_iff hK).mpr;
+      intro Ω' hΩ';
+      apply ih.mp;
+      simp [Satisfies.box_def] at h;
+      exact h Ω' hΩ';
+    . intro h Ω' hΩ';
+      apply ih.mpr;
+      simp [Set.subset_def, CanonicalModel.frame_def] at hΩ';
+      exact hΩ' h;
+  -/
+
+end Kripke
+
+end LO.Modal.Standard
