Logic/Modal/Standard/Kripke/Reducible.lean
@@ -7,12 +7,11 @@ namespace Kripke
 
 variable {W α : Type*} [DecidableEq α]
 variable {Λ₁ Λ₂ : AxiomSet α} {P₁ P₂ : Frame W α → Prop}
-variable (𝔽Λ₁ : AxiomSetFrameClass W Λ₁) (𝔽Λ₂ : AxiomSetFrameClass W Λ₂)
-variable [hSound₁ : Sound Λ₁ 𝔽Λ₁] [hSound₂ : Sound Λ₂ 𝔽Λ₂]
-variable [hComp₁ : Complete Λ₁ 𝔽Λ₁] [hComp₂ : Complete Λ₂ 𝔽Λ₂]
+variable [hSound₁ : Sound Λ₁ 𝔽(Λ₁, W)] [hSound₂ : Sound Λ₂ 𝔽(Λ₂, W)]
+variable [hComp₁ : Complete Λ₁ 𝔽(Λ₁, W)] [hComp₂ : Complete Λ₂ 𝔽(Λ₂, W)]
 variable (hDec₁ : AxiomSetDefinability W Λ₁ P₁) (hDec₂ : AxiomSetDefinability W Λ₂ P₂)
 
-lemma reducible_of_subset_axiomSetFrameClass (hs : 𝔽Λ₂.frameclass ⊆ 𝔽Λ₁.frameclass) : Λ₁ ≤ₛ Λ₂ := by
+lemma reducible_of_subset_axiomSetFrameClass (hs : 𝔽(Λ₂, W) ⊆ 𝔽(Λ₁, W)) : Λ₁ ≤ₛ Λ₂ := by
   apply System.reducible_iff.mpr;
   intro p hp;
   apply hComp₂.complete;
@@ -20,24 +19,24 @@ lemma reducible_of_subset_axiomSetFrameClass (hs : 𝔽Λ₂.frameclass ⊆ 𝔽
   exact hSound₁.sound hp F (hs hF);
 
 lemma reducible_of_definability (hs : ∀ {F : Frame W α}, P₂ F → P₁ F) : Λ₁ ≤ₛ Λ₂ := by
-  apply reducible_of_subset_axiomSetFrameClass 𝔽Λ₁ 𝔽Λ₂;
+  apply reducible_of_subset_axiomSetFrameClass (W := W);
   intro h hF;
   apply iff_definability_memAxiomSetFrameClass hDec₁ |>.mp;
   exact hs $ iff_definability_memAxiomSetFrameClass hDec₂ |>.mpr hF;
 
-lemma equiv_of_eq_axiomSetFrameClass (heq : 𝔽Λ₁.frameclass = 𝔽Λ₂.frameclass) : Λ₁ =ₛ Λ₂ := by
+lemma equiv_of_eq_axiomSetFrameClass (heq : 𝔽(Λ₁, W) = 𝔽(Λ₂, W)) : Λ₁ =ₛ Λ₂ := by
   apply System.Equiv.antisymm_iff.mpr;
   constructor;
-  . exact reducible_of_subset_axiomSetFrameClass 𝔽Λ₁ 𝔽Λ₂ heq.symm.subset;
-  . exact reducible_of_subset_axiomSetFrameClass 𝔽Λ₂ 𝔽Λ₁ heq.subset;
+  . exact reducible_of_subset_axiomSetFrameClass heq.symm.subset;
+  . exact reducible_of_subset_axiomSetFrameClass heq.subset;
 
 lemma equiv_of_iff_definability (h : ∀ {F : Frame W α}, P₁ F ↔ P₂ F) : Λ₁ =ₛ Λ₂ := by
   apply System.Equiv.antisymm_iff.mpr;
   constructor;
-  . apply reducible_of_definability 𝔽Λ₁ 𝔽Λ₂ hDec₁ hDec₂;
+  . apply reducible_of_definability hDec₁ hDec₂;
     intro F hF;
     exact h.mpr hF;
-  . apply reducible_of_definability 𝔽Λ₂ 𝔽Λ₁ hDec₂ hDec₁;
+  . apply reducible_of_definability hDec₂ hDec₁;
     intro F hF;
     exact h.mp hF;
 
